src/lib/state/DY.Lib.State.Tagged.fst
@@ -313,6 +313,32 @@ let get_tagged_state_same_trace tag prin sess_id tr =
   reveal_opaque (`%get_tagged_state) (get_tagged_state)
 
 
+val get_tagged_state_state_was_set:
+  tag:string -> 
+  prin:principal -> sess_id:state_id -> tr:trace ->
+  Lemma
+  (ensures (
+    let (opt_content, tr_out) = get_tagged_state tag prin sess_id tr in
+    tr == tr_out /\ (
+      match opt_content with
+      | None -> True
+      | Some content -> (
+         tagged_state_was_set tr tag prin sess_id content
+      )
+    )
+  )
+  )
+  [SMTPat (get_tagged_state tag prin sess_id tr)]
+let get_tagged_state_state_was_set tag prin sess_id tr =
+  reveal_opaque (`%get_tagged_state) (get_tagged_state);
+  reveal_opaque (`%tagged_state_was_set) (tagged_state_was_set);
+  match get_tagged_state tag prin sess_id tr with
+  | (None, _) -> ()
+  | (Some _, _) -> (
+    let (Some full_cont_bytes, _) = get_state prin sess_id tr in
+    serialize_parse_inv_lemma #bytes tagged_state full_cont_bytes    
+  )
+
 val get_tagged_state_invariant:
   {|protocol_invariants|} ->
   tag:string -> spred:local_bytes_state_predicate tag ->
