src/lib/event/DY.Lib.Event.Typed.fst
@@ -226,10 +226,10 @@ val event_triggered_at_implies_trace_event_at:
   tr:trace -> i:timestamp -> prin:principal -> e:a  ->
   Lemma
   (requires event_triggered_at tr i prin e)
-  (ensures (
+  (ensures
     get_event_at tr i == Event prin ev.tag (serialize a e) /\
     parse #bytes a (serialize a e) == Some e
-  ))
+  )
   [SMTPat (event_triggered_at tr i prin e)]
 let event_triggered_at_implies_trace_event_at #a #ev tr i prin e =
   reveal_opaque (`%event_triggered_at) (event_triggered_at #a);
